First try at a rewrite of HMAC

code/experimental/hmac/Hacl.HMAC.fst
@@ -6,182 +6,150 @@ open FStar.HyperStack
 open FStar.ST
 open FStar.Buffer
 
+open Hacl.Cast
 open Hacl.UInt8
 open Hacl.UInt32
 open FStar.UInt32
 
-open Hacl.Cast
-open Hacl.SBuffer
-open Hacl.Operations
-open Hacl.Conversions
+open Hacl.Utils.Experimental
 
+
+(* Definition of aliases for modules *)
 module U8 = FStar.UInt8
-module S8 = Hacl.UInt8
 module U32 = FStar.UInt32
-module S32 = Hacl.UInt32
 module U64 = FStar.UInt64
+
+module S8 = Hacl.UInt8
+module S32 = Hacl.UInt32
 module S64 = Hacl.UInt64
-module SB = Hacl.SBuffer
-module FB = FStar.Buffer
 
-module HM = Hash.SHA2.L256
+module Buffer = FStar.Buffer
+module Cast = Hacl.Cast
+module Utils = Hacl.Utils.Experimental
 
-
-(* Define base types *)
-let s8 = Hacl.UInt8.t
-let u32 = FStar.UInt32.t
-let s32 = Hacl.UInt32.t
-let u64 = FStar.UInt64.t
-let s64 = Hacl.UInt64.t
-let uint32s = Hacl.SBuffer.u32s
-let bytes = Hacl.SBuffer.u8s
+module Hash = Hacl.Hash.SHA2.L256
 
 
-(* Define operators *)
-let op_Plus_At = U32.add_mod
+(* Definition of base types *)
+let uint8_t   = FStar.UInt8.t
+let uint32_t  = FStar.UInt32.t
+let uint64_t  = FStar.UInt64.t
+
+let suint8_t  = Hacl.UInt8.t
+let suint32_t = Hacl.UInt32.t
+let suint64_t = Hacl.UInt64.t
+
+let suint32_p = Buffer.buffer suint32_t
+let suint8_p  = Buffer.buffer suint8_t
+
+
+(* Definitions of aliases for functions *)
+let u8_to_s8 = Cast.uint8_to_sint8
+let u32_to_s32 = Cast.uint32_to_sint32
+let u32_to_s64 = Cast.uint32_to_sint64
+let s32_to_s8  = Cast.sint32_to_sint8
+let s32_to_s64 = Cast.sint32_to_sint64
+let u64_to_s64 = Cast.uint64_to_sint64
+
+
+
+//
+// HMAC
+//
 
 
 (* Define parameters *)
-let hash = HM.sha256
-let hashsize = HM.hashsize
-let blocksize = HM.blocksize
-let hl = hashsize
-let bl = blocksize
+inline_for_extraction let hash = Hash.sha256
+inline_for_extraction let hashsize = Hash.hashsize
+inline_for_extraction let blocksize = Hash.blocksize
 
+
+(* Size and positions of objects in memb *)
+inline_for_extraction let size_ipad = blocksize
+inline_for_extraction let size_opad = blocksize
+inline_for_extraction let size_okey = blocksize
+inline_for_extraction let size_s3   = blocksize +^ blocksize
+inline_for_extraction let size_s6   = blocksize +^ blocksize
+inline_for_extraction let size_memb = size_ipad +^ size_opad +^ size_okey +^ size_s3 +^ size_s6
+
+inline_for_extraction let pos_ipad  = 0ul
+inline_for_extraction let pos_opad  = pos_ipad +^ blocksize
+inline_for_extraction let pos_okey  = pos_opad +^ blocksize
+inline_for_extraction let pos_s3    = pos_okey +^ blocksize
+inline_for_extraction let pos_s6    = pos_s3 +^ blocksize
 
 
 (* Define a function to wrap the key length after bl bits *)
-val wrap_key : (okey   :bytes{length okey = U32.v bl}) ->
-               (key    :bytes{length key % (U32.v bl) = 0 /\ disjoint okey key}) ->
-               (keylen :u32  {U32.v keylen <= length key /\ U32.v keylen + 8 < pow2 32})
-  -> STL unit
-        (requires (fun h -> live h okey /\ live h key))
+private val hmac_wrap_key:
+  okey   :suint8_p{length okey = U32.v blocksize} ->
+  key    :suint8_p ->
+  keylen :uint32_t{U32.v keylen <= length key /\ U32.v keylen + 8 < pow2 32} ->
+  Stack unit
+        (requires (fun h0 -> live h0 okey /\ live h0 key))
         (ensures  (fun h0 _ h1 -> live h1 okey /\ live h1 key /\ modifies_1 okey h0 h1))
 
-let wrap_key okey key keylen =
-  if gt keylen bl then
+let hmac_wrap_key okey key keylen =
+  if U32.(keylen >^ blocksize) then
     hash okey key keylen
   else
     blit key 0ul okey 0ul keylen
 
 
 
-(* Size and positions of objects in memb *)
-let size_ipad = bl
-let size_opad = bl
-let size_okey = bl
-let size_s3 = bl +@ bl
-let size_s6 = bl +@ bl
-let size_memb = size_ipad +@ size_opad +@ size_okey +@ size_s3 +@ size_s6
+val hmac:
+  mac     :suint8_p{length mac = U32.v hashsize} ->
+  key     :suint8_p ->
+  keylen  :uint32_t{U32.v keylen <= length key} ->
+  data    :suint8_p ->
+  datalen :uint32_t{U32.v datalen <= length data /\ U32.v datalen + U32.v blocksize <= pow2 32} ->
+  Stack unit
+        (requires (fun h -> live h mac /\ live h key /\ live h data ))
+        (ensures  (fun h0 r h1 -> live h1 mac /\ modifies_1 mac h0 h1))
 
-let pos_ipad = 0ul
-let pos_opad = bl
-let pos_okey = bl +@ bl
-let pos_s3 = bl +@ bl +@ bl
-let pos_s6 = bl +@ bl +@ bl +@ bl +@ bl
+let hmac mac key keylen data datalen =
 
+  (* Push a new memory frame *)
+  (**) push_frame();
 
-#reset-options "--z3rlimit 20"
+  (* Allocate memory for the padding *)
+  let memb = Buffer.create (uint8_to_sint8 0uy) size_memb in
 
+  (* Allocate and set initial values for ipad and opad *)
+  let ipad = Buffer.create (uint8_to_sint8 0x36uy) size_ipad in
+  let opad = Buffer.create (uint8_to_sint8 0x5cuy) size_opad in
 
-(* Define the internal function *)
-val hmac_core' :  (memb    :bytes {length memb = U32.v size_memb}) ->
-                  (mac     :bytes {length mac = U32.v hl /\ disjoint mac memb }) ->
-                  (key     :bytes {length key % (U32.v bl) = 0 /\ disjoint key memb }) ->
-                  (keylen  :u32   {U32.v keylen <= length key}) ->
-                  (data    :bytes {length data % (U32.v bl) = 0 /\ disjoint data memb /\ disjoint mac data }) ->
-                  (datalen :u32   {U32.v datalen <= length data /\ U32.v datalen + U32.v bl <= pow2 32})
-                  -> STL unit
-                        (requires (fun h -> live h memb /\ live h mac /\ live h data /\ live h key))
-                        (ensures  (fun h0 r h1 -> live h1 memb /\ live h1 mac /\ modifies_2 memb mac h0 h1))
+  (* Allocate memory for the wrapped key location *)
+  let okey = Buffer.create (uint8_to_sint8 0uy) size_okey in
 
-let hmac_core' memb mac key keylen data datalen =
-
-  (* Define ipad and opad *)
-  (**) let h0 = ST.get() in
-
-  (* Set initial values for ipad and opad *)
-  let ipad = sub memb pos_ipad size_ipad in
-  setall ipad (uint8_to_sint8 0x36uy) size_ipad;
-  let opad = sub memb pos_opad size_opad in
-  setall opad (uint8_to_sint8 0x5cuy) size_opad;
-
-  (* Create the wrapped key location *)
-  let okey = sub memb pos_okey size_okey in
-
-  (* Create the working emplacements *)
-  let s3 = sub memb pos_s3 size_s3 in
-  let s6 = sub memb pos_s6 size_s6 in
+  (* Allocate memory for working emplacements *)
+  let s3 = Buffer.create (uint8_to_sint8 0uy) size_s3 in
+  let s6 = Buffer.create (uint8_to_sint8 0uy) size_s6 in
 
   (* Step 1: make sure the key has the proper length *)
-  wrap_key okey key keylen;
+  hmac_wrap_key okey key keylen;
 
   (* Step 2: xor "result of step 1" with ipad *)
-  xor_bytes ipad okey bl;
+  Utils.xor_bytes ipad okey blocksize;
   let s2 = ipad in
 
   (* Step 3: append data to "result of step 2" *)
-  blit s2 0ul s3 0ul bl;
-  blit data 0ul s3 bl bl;
+  Buffer.blit s2 0ul s3 0ul blocksize;
+  Buffer.blit data 0ul s3 blocksize blocksize;
 
   (* Step 4: apply H to "result of step 3" *)
   let s4 = s2 in
-  hash s4 s3 (bl +@ datalen);
+  hash s4 s3 (blocksize +^ datalen);
 
   (* Step 5: xor "result of step 1" with opad *)
-  xor_bytes okey opad bl;
+  Utils.xor_bytes okey opad blocksize;
   let s5 = okey in
 
   (* Step 6: append "result of step 4" to "result of step 5" *)
-  blit s5 0ul s6 0ul bl;
-  blit s4 0ul s6 bl bl;
-
-  (**) let h1 = ST.get() in
-  (**) assert(modifies_1 memb h0 h1);
+  Buffer.blit s5 0ul s6 0ul blocksize;
+  Buffer.blit s4 0ul s6 blocksize blocksize;
 
   (* Step 7: apply H to "result of step 6" *)
-  hash mac s6 (bl +@ hl);
+  hash mac s6 (blocksize +^ hashsize);
 
-  (**) let h2 = ST.get() in
-  (**) assert(modifies_2 memb mac h0 h2);
-  (**) assert(live h2 memb);
-  (**) assert(live h2 mac)
-
-
-
-
-(* Define the main function *)
-val hmac_core : (mac     :bytes {length mac = U32.v hl}) ->
-                (key     :bytes {length key % (U32.v bl) = 0}) ->
-                (keylen  :u32   {U32.v keylen <= length key}) ->
-                (data    :bytes {length data % (U32.v bl) = 0 /\ disjoint mac data}) ->
-                (datalen :u32   {U32.v datalen <= length data /\ U32.v datalen + U32.v bl <= pow2 32})
-  -> STL unit
-        (requires (fun h -> live h mac /\ live h data /\ live h key))
-        (ensures  (fun h0 r h1 -> live h1 mac /\ modifies_1 mac h0 h1))
-
-let hmac_core mac key keylen data datalen =
-
-  (* Push a new frame *)
-  (**) push_frame();
-
-  let memblen = size_memb in
-  let memb = create (uint8_to_sint8 0uy) memblen in
-
-  hmac_core' memb mac key keylen data datalen;
-
-  (* Pop the current frame *)
+  (* Pop the memory frame *)
   (**) pop_frame()
-
-
-(* Exposing SHA2-256 for test vectors *)
-val hmac_sha256 : (mac     :bytes {length mac = U32.v hl}) ->
-                  (key     :bytes {length key % (U32.v bl) = 0}) ->
-                  (keylen  :u32   {U32.v keylen <= length key}) ->
-                  (data    :bytes {length data % (U32.v bl) = 0 /\ disjoint mac data}) ->
-                  (datalen :u32   {U32.v datalen <= length data /\ U32.v datalen + U32.v bl <= pow2 32})
-  -> STL unit
-        (requires (fun h -> live h mac /\ live h data /\ live h key))
-        (ensures  (fun h0 r h1 -> live h1 mac /\ modifies_1 mac h0 h1))
-
-let hmac_sha256 mac key keylen data datalen = hmac_core mac key keylen data datalen
